Prove wp_index__getKeys and wp_index__DoGC
Delete gc_proof.v

etc/update-goose.py
@@ -257,7 +257,6 @@ def main():
             mvcc_dir,
             "./txn",
             "./index",
-            "./gc",
             "./tuple",
             "./wrbuf",
             "./tid",
